src/x86/instrrules/out.v
@@ -3,7 +3,7 @@ Require Import x86.instrrules.core.
 Import x86.instrrules.core.instrruleconfig.
 
 (** Special case for negation *)
-Lemma OUT_R_rule c d :
+Lemma OUT_R_rule (c: BYTE) d :
   |-- basic
-      (BYTEregIs AL d) (OUT false c) (outOP c d) (BYTEregIs AL d).
+      (BYTEregIs AL d) (OUT c, AL) (outOP (zeroExtend 8 c) d) (BYTEregIs AL d).
 Proof. Admitted.
