src/x86/instrrules/ret.v
@@ -2,8 +2,6 @@
 Require Import x86.instrrules.core.
 Import x86.instrrules.core.instrruleconfig.
 
-Require Import safe (* for [safe] *).
-
 Lemma RET_rule p' (sp:DWORD) (offset:WORD) (p q: DWORD) O :
   let sp':DWORD := addB (sp+#4) (zeroExtend 16 offset) in
   |-- (
